p256: clean up point_double

code/ecdsap256/Hacl.Impl.P256.PointDouble.fst
@@ -1,485 +1,176 @@
 module Hacl.Impl.P256.PointDouble
 
+open FStar.Mul
 open FStar.HyperStack.All
 open FStar.HyperStack
 module ST = FStar.HyperStack.ST
-
-open FStar.Mul
-open FStar.Math.Lemmas
-open FStar.Tactics
-open FStar.Tactics.Canon
 
 open Lib.IntTypes
 open Lib.Buffer
 
 open Hacl.Impl.P256.Field
-open Hacl.Spec.P256.Math
 
 module S = Spec.P256
 module SM = Hacl.Spec.P256.MontgomeryMultiplication
+module SL = Hacl.Spec.P256.Math
 
-#set-options "--z3rlimit 300 --ifuel 0 --fuel 0"
+#set-options "--z3rlimit 50 --ifuel 0 --fuel 0"
 
-val lemma_x3_0: x: int -> y: int -> z: int -> Lemma (
-  ((3 * (x - (z * z % S.prime)) * (x + (z * z % S.prime)) % S.prime) * (3 * (x - (z * z % S.prime)) * (x + (z * z % S.prime)) % S.prime)  - 8 * (x * (y * y % S.prime) % S.prime)) % S.prime ==  ((3 * (x - (z * z % S.prime)) * (x + (z * z % S.prime)) % S.prime) * (3 * (x - (z * z % S.prime)) * (x + (z * z % S.prime)) % S.prime) - 8 * x * y * y) % S.prime)
-
-let lemma_x3_0 x y z =
-  let t0 = (3 * (x - (z * z % S.prime)) * (x + (z * z % S.prime)) % S.prime) in
-  calc (==)
-  {
-    (t0 * t0 - 8 * (x * (y * y % S.prime) % S.prime)) % S.prime;
-    (==) {lemma_mod_mul_distr_r x (y * y) S.prime}
-    (t0 * t0 - 8 * ((x * (y * y)) % S.prime)) % S.prime;
-    (==) {assert_by_tactic (x * (y * y) == x * y * y) canon}
-    (t0 * t0 - 8 * (x * y * y % S.prime)) % S.prime;
-    (==) {lemma_mod_sub_distr (t0 * t0) (8 * (x * y * y % S.prime)) S.prime}
-    (t0 * t0 - (8 * (x * y * y % S.prime)) % S.prime) % S.prime;
-    (==) {lemma_mod_mul_distr_r 8 (x * y * y) S.prime}
-    (t0 * t0 - (8 * (x * y * y)) % S.prime) % S.prime;
-    (==) {assert_by_tactic (8 * (x * y * y) == 8 * x * y * y) canon}
-    (t0 * t0 - (8 * x * y * y) % S.prime) % S.prime;
-    (==) {lemma_mod_sub_distr (t0 * t0) (8 * x * y * y) S.prime}
-    (t0 * t0 - 8 * x * y * y) % S.prime;
-
-  }
-
-
-val lemma_x3_1: a: int -> b: int -> Lemma (((a % S.prime) * (a % S.prime) - b) % S.prime == (a * a - b) % S.prime)
-
-let lemma_x3_1 a b =
-  calc (==)
-  {
-    ((a % S.prime) * (a % S.prime) - b) % S.prime;
-    (==) {lemma_mod_add_distr (- b) ((a % S.prime) * (a % S.prime)) S.prime}
-    ((a % S.prime) * (a % S.prime) % S.prime - b) % S.prime;
-    (==) {lemma_mod_mul_distr_l a (a % S.prime) S.prime; lemma_mod_mul_distr_r a a S.prime}
-    (a * a % S.prime - b) % S.prime;
-    (==) {lemma_mod_add_distr (- b) (a * a) S.prime}
-    (a * a - b) % S.prime;
-  }
-
-
-val lemma_x3: x: int -> y: int -> z: int -> Lemma (
-  ((3 * (x - (z * z % S.prime)) * (x + (z * z % S.prime)) % S.prime) * (3 * (x - (z * z % S.prime)) * (x + (z * z % S.prime)) % S.prime) - 8 * (x * (y * y % S.prime) % S.prime)) % S.prime ==
-  ((3 * (x - z * z) * (x + z * z)) * (3 * (x - z * z) * (x + z * z)) - 8 * x * (y * y)) % S.prime
-)
-
-let lemma_x3 x y z =
-  lemma_x3_0 x y z;
-
-  calc (==)
-  {
-    (
-      (3 * (x - (z * z % S.prime)) * (x + (z * z % S.prime)) % S.prime) *
-      (3 * (x - (z * z % S.prime)) * (x + (z * z % S.prime)) % S.prime) - 8 * x * y * y) % S.prime;
-
-    (==) {lemma_mod_mul_distr_l (3 * (x - (z * z % S.prime))) (x + (z * z % S.prime)) S.prime}
-
-    (
-      (3 * (x - (z * z % S.prime)) % S.prime * (x + (z * z % S.prime)) % S.prime) *
-      (3 * (x - (z * z % S.prime)) % S.prime * (x + (z * z % S.prime)) % S.prime) - 8 * x * y * y) % S.prime;
-
-  (==) {lemma_mod_mul_distr_r 3 (x - (z * z % S.prime)) S.prime}
-
-     (
-       (3 * ((x - (z * z % S.prime)) % S.prime) % S.prime * (x + (z * z % S.prime)) % S.prime) *
-       (3 * ((x - (z * z % S.prime)) % S.prime) % S.prime * (x + (z * z % S.prime)) % S.prime) - 8 * x * y * y) % S.prime;
-
-   (==) {lemma_mod_sub_distr x (z * z) S.prime}
-
-     (
-       (3 * ((x - z * z) % S.prime) % S.prime * (x + (z * z % S.prime)) % S.prime) *
-       (3 * ((x - z * z) % S.prime) % S.prime * (x + (z * z % S.prime)) % S.prime) - 8 * x * y * y) % S.prime;
-
-  (==) {lemma_mod_mul_distr_r 3 (x - (z * z)) S.prime}
-
-     (
-       (3 * ((x - z * z)) % S.prime * (x + (z * z % S.prime)) % S.prime) *
-       (3 * ((x - z * z)) % S.prime * (x + (z * z % S.prime)) % S.prime) - 8 * x * y * y) % S.prime;
-
-  (==) {lemma_mod_mul_distr_l (3 * (x - z * z)) (x + (z * z % S.prime)) S.prime}
-
-     (
-       (3 * (x - z * z) * (x + (z * z % S.prime)) % S.prime) *
-       (3 * (x - z * z) * (x + (z * z % S.prime)) % S.prime) - 8 * x * y * y) % S.prime;
-
-  (==) {lemma_mod_mul_distr_r (3 * (x - z * z)) (x + (z * z % S.prime)) S.prime;
-       lemma_mod_add_distr x (z * z) S.prime;
-       lemma_mod_mul_distr_r (3 * (x - z * z)) (x + z * z) S.prime}
-
-    (
-      (3 * (x - z * z) * (x + (z * z)) % S.prime) *
-      (3 * (x - z * z) * (x + (z * z)) % S.prime) - 8 * x * y * y) % S.prime;
-
-  (==) {lemma_x3_1 (3 * (x - z * z) * (x + (z * z))) (8 * x * y * y)}
-
-    (
-      (3 * (x - z * z) * (x + z * z)) *
-      (3 * (x - z * z) * (x + z * z)) - 8 * x * y * y) % S.prime;
-
- (==) {assert_by_tactic (8 * x * y * y == 8 * x * (y * y)) canon}
-     (
-      (3 * (x - z * z) * (x + z * z)) *
-      (3 * (x - z * z) * (x + z * z)) - 8 * x * (y * y)) % S.prime;
-}
-
-
-val y3_lemma_0: x: int ->  y: int -> z: int ->  t0: int -> Lemma (
-   (t0 - 8 * (y * y % S.prime) * (y * y % S.prime)) % S.prime == (t0 - 8 * y * y * y * y) % S.prime)
-
-let y3_lemma_0 x y z t0 =
-  calc (==) {
-    (t0 - 8 * (y * y % S.prime) * (y * y % S.prime)) % S.prime;
-  (==) {lemma_mod_sub_distr t0 (8 * (y * y % S.prime) * (y * y % S.prime)) S.prime}
-    (t0 - (8 * (y * y % S.prime) * (y * y % S.prime)) % S.prime) % S.prime;
-  (==) {lemma_mod_mul_distr_r (8 * (y * y % S.prime)) (y * y) S.prime}
-    (t0 - (8 * (y * y % S.prime) * (y * y)) % S.prime) % S.prime;
-  (==) {lemma_mod_mul_distr_r (8 * (y * y)) (y * y) S.prime}
-    (t0 - (8 * (y * y) * (y * y)) % S.prime) % S.prime;
-  (==) {assert_by_tactic (8 * (y * y) * (y * y) == 8 * y * y * y * y) canon}
-    (t0 - (8 * y * y * y * y) % S.prime) % S.prime;
-  (==) {lemma_mod_sub_distr t0 (8 * y * y * y * y) S.prime}
-    (t0 - (8 * y * y * y * y)) % S.prime;
-  (==) {assert_by_tactic (t0 - (8 * y * y * y * y) == t0 - 8 * y * y * y * y) canon}
-    (t0 - 8 * y * y * y * y) % S.prime;
-  }
-
-
-val y3_lemma_1: x: int ->  y: int -> z: int ->
-  Lemma (3 * (x - (z * z % S.prime)) * (x + (z * z % S.prime)) % S.prime == 3 * (x + z * z) * (x - z * z)  % S.prime)
-
-let sym_decidable (#a:eqtype) (x y:a) : Lemma (requires y = x) (ensures x == y) = ()
-
-let y3_lemma_1 x y z =
-  calc (==)
-  {
-    3 * (x - (z * z % S.prime)) * (x + (z * z % S.prime)) % S.prime;
-    (==) {lemma_mod_mul_distr_r (3 * (x - (z * z % S.prime))) (x + (z * z % S.prime)) S.prime}
-      3 * (x - (z * z % S.prime)) * ((x + (z * z % S.prime)) % S.prime) % S.prime;
-    (==) {lemma_mod_add_distr x (z * z) S.prime}
-      3 * (x - (z * z % S.prime)) * ((x + z * z) % S.prime) % S.prime;
-    (==) {lemma_mod_mul_distr_r (3 * (x - (z * z % S.prime))) (x + z * z) S.prime}
-      3 * (x - (z * z % S.prime)) * (x + z * z) % S.prime;
-    (==) {assert_by_tactic (3 * (x - (z * z % S.prime)) * (x + z * z) == 3 * (x + z * z) * (x - (z * z % S.prime))) canon}
-      3 * (x + z * z) * (x - (z * z % S.prime)) % S.prime;
-    (==) {lemma_mod_mul_distr_r (3 * (x + z * z)) (x - (z * z % S.prime)) S.prime}
-      3 * (x + z * z) * ((x - (z * z % S.prime))  % S.prime)  % S.prime;
-    (==) {lemma_mod_sub_distr x (z * z) S.prime}
-      3 * (x + z * z) * ((x - z * z) % S.prime)  % S.prime;
-    (==) { _ by FStar.Tactics.(mapply (`sym_decidable); mapply (`lemma_mod_mul_distr_r)) }
-      3 * (x + z * z) * (x - z * z)  % S.prime;
-    }
-
-
-val lemma_y3: x: int -> y: int -> z: int -> x3: int -> Lemma (
-  ((3 * (x - (z * z % S.prime)) * (x + (z * z % S.prime)) % S.prime) *  ((4 * (x * (y * y % S.prime) % S.prime) % S.prime) - x3) - 8 * (y * y % S.prime) * (y * y % S.prime)) % S.prime == (3 * (x - z * z) * (x + z * z) *  (4 * x * (y * y) - x3) - 8 * (y * y) * (y * y)) % S.prime)
-
-
-let lemma_y3 x y z x3 =
-  let t = ((3 * (x - (z * z % S.prime)) * (x + (z * z % S.prime)) % S.prime) *  ((4 * (x * (y * y % S.prime) % S.prime) % S.prime) - x3) - 8 * (y * y % S.prime) * (y * y % S.prime)) % S.prime in
-  let t0 = (3 * (x - (z * z % S.prime)) * (x + (z * z % S.prime)) % S.prime) *  ((4 * (x * (y * y % S.prime) % S.prime) % S.prime) - x3) in
-  assert(t == (t0 - 8 * (y * y % S.prime) * (y * y % S.prime)) % S.prime);
-
-  y3_lemma_0 x y z t0;
-  y3_lemma_1 x y z;
-
-
-  calc (==)
-  {
-      4 * (x * (y * y % S.prime) % S.prime) % S.prime;
-    (==) {lemma_mod_mul_distr_r x (y * y) S.prime}
-       4 * ((x * (y * y)) % S.prime) % S.prime;
-    (==) {assert_by_tactic (x * (y * y) == x * y * y) canon}
-      (4 * ((x * y * y) % S.prime)) % S.prime;
-    (==) {lemma_mod_mul_distr_r 4 (x * y * y) S.prime}
-      (4 * (x * y * y)) % S.prime;
-    (==) {assert_by_tactic (4 * (x * y * y) == 4 * x * y * y) canon}
-      4 * x * y * y % S.prime;
-
-   };
-
-  calc (==)
-  {
-    ((3 * (x + z * z) * (x - z * z)  % S.prime) *  (4 * x * y * y % S.prime - x3) - 8 * y * y * y * y) % S.prime;
-    (==) {lemma_mod_add_distr (- 8 * y * y * y * y) ((3 * (x + z * z) * (x - z * z)  % S.prime) *  (4 * x * y * y % S.prime - x3)) S.prime}
-    ((((3 * (x + z * z) * (x - z * z)) % S.prime) *  (4 * x * y * y % S.prime - x3)) % S.prime - 8 * y * y * y * y) % S.prime;
-    (==) {lemma_mod_mul_distr_l (3 * (x + z * z) * (x - z * z))  (4 * x * y * y % S.prime - x3) S.prime}
-    (((3 * (x + z * z) * (x - z * z)) *  (4 * x * y * y % S.prime - x3)) % S.prime - 8 * y * y * y * y) % S.prime;
-    (==) {lemma_mod_mul_distr_r (3 * (x + z * z) * (x - z * z)) (4 * x * y * y % S.prime - x3) S.prime}
-    (((3 * (x + z * z) * (x - z * z)) *  ((4 * x * y * y % S.prime - x3) % S.prime)) % S.prime - 8 * y * y * y * y) % S.prime;
-    (==) {lemma_mod_add_distr (- x3) (4 * x * y * y) S.prime}
-    (((3 * (x + z * z) * (x - z * z)) *  ((4 * x * y * y - x3) % S.prime)) % S.prime - 8 * y * y * y * y) % S.prime;
-    (==) {lemma_mod_mul_distr_r (3 * (x + z * z) * (x - z * z)) (4 * x * y * y - x3) S.prime}
-    ((3 * (x + z * z) * (x - z * z) *  (4 * x * y * y - x3)) % S.prime - 8 * y * y * y * y) % S.prime;
-    (==) {lemma_mod_add_distr (- 8 * y * y * y * y) (3 * (x + z * z) * (x - z * z) *  (4 * x * y * y - x3)) S.prime}
-    (3 * (x + z * z) * (x - z * z) *  (4 * x * y * y - x3) - 8 * y * y * y * y) % S.prime;
-    (==) {assert_by_tactic (8 * y * y * y * y == 8 * (y * y) * (y * y)) canon}
-    (3 * (x + z * z) * (x - z * z) *  (4 * x * y * y - x3) - 8 * (y * y) * (y * y)) % S.prime;
-    (==) {assert_by_tactic (4 * x * y * y == 4 * x * (y * y)) canon}
-    (3 * (x + z * z) * (x - z * z) *  (4 * x * (y * y) - x3) - 8 * (y * y) * (y * y)) % S.prime;
-    (==) {assert_by_tactic ((3 * (x + z * z) * (x - z * z) *  (4 * x * (y * y) - x3) - 8 * (y * y) * (y * y)) == (3 * (x - z * z) * (x + z * z) *  (4 * x * (y * y) - x3) - 8 * (y * y) * (y * y))) canon}
-    (3 * (x - z * z) * (x + z * z) *  (4 * x * (y * y) - x3) - 8 * (y * y) * (y * y)) % S.prime;
-
-  }
-
-
-val lemma_z3: x: int -> y: int -> z: int -> Lemma
-  (((y + z) * (y + z) - (y * y % S.prime) - (z * z % S.prime)) % S.prime == ((y + z) * (y + z) - z * z - y * y) % S.prime)
-
-
-let lemma_z3 x y z =
-  let t = ((y + z) * (y + z) - (y * y % S.prime) - (z * z % S.prime)) % S.prime in
-
-  calc (==)
-    {
-      ((y + z) * (y + z) - (y * y % S.prime) - (z * z % S.prime)) % S.prime;
-      (==) {lemma_mod_sub_distr ((y + z) * (y + z) - (y * y % S.prime)) (z * z) S.prime}
-      ((y + z) * (y + z) - (y * y % S.prime) - z * z) % S.prime;
-      (==) {lemma_mod_sub_distr ((y + z) * (y + z) - z * z) (y * y) S.prime}
-      ((y + z) * (y + z) - z * z - y * y) % S.prime;}
-
-
-val point_double_a_b_g: p: point -> alpha: felem -> beta: felem -> gamma: felem -> delta: felem -> tempBuffer: lbuffer uint64 (size 12) ->
+inline_for_extraction noextract
+val point_double_a_b_g_d:
+    p:point
+  -> alpha:felem -> beta:felem -> gamma:felem -> delta:felem
+  -> tmp:felem ->
   Stack unit
-    (requires fun h ->
-      live h p /\ live h alpha /\ live h beta /\ live h gamma /\ live h delta /\ live h tempBuffer /\
-      LowStar.Monotonic.Buffer.all_disjoint [loc p; loc alpha; loc beta; loc gamma; loc delta; loc tempBuffer] /\
-      as_nat h (gsub p (size 8) (size 4)) < S.prime /\
-      as_nat h (gsub p (size 0) (size 4)) < S.prime /\
-      as_nat h (gsub p (size 4) (size 4)) < S.prime
-    )
-    (ensures fun h0 _ h1 -> modifies (loc alpha |+| loc beta |+| loc gamma |+| loc delta |+| loc tempBuffer) h0 h1 /\
-      (
-	let x = SM.from_mont (as_nat h0 (gsub p (size 0) (size 4))) in
-	let y = SM.from_mont (as_nat h0 (gsub p (size 4) (size 4))) in
-	let z = SM.from_mont (as_nat h0 (gsub p (size 8) (size 4))) in
-	as_nat h1 delta = SM.to_mont (z * z % S.prime) /\
-	as_nat h1 gamma = SM.to_mont (y * y % S.prime) /\
-	as_nat h1 beta = SM.to_mont (x * SM.from_mont(as_nat h1 gamma) % S.prime) /\
-	as_nat h1 alpha = SM.to_mont (3 * (x - SM.from_mont (as_nat h1 delta)) * (x + SM.from_mont (as_nat h1 delta)) % S.prime)
-      )
-    )
+  (requires fun h ->
+    live h p /\ live h alpha /\ live h beta /\
+    live h gamma /\ live h delta /\ live h tmp /\
+    LowStar.Monotonic.Buffer.all_disjoint
+      [loc p; loc alpha; loc beta; loc gamma; loc delta; loc tmp] /\
+    point_inv h p)
+  (ensures fun h0 _ h1 ->
+    modifies (loc alpha |+| loc beta |+| loc gamma |+| loc delta |+| loc tmp) h0 h1 /\
+    as_nat h1 alpha < S.prime /\ as_nat h1 beta < S.prime /\
+    as_nat h1 gamma < S.prime /\ as_nat h1 delta < S.prime /\
+   (let x, y, z = SM.from_mont_point (as_point_nat h0 p) in
+    fmont_as_nat h1 delta = S.fmul z z /\
+    fmont_as_nat h1 gamma = S.fmul y y /\
+    fmont_as_nat h1 beta = S.fmul x (fmont_as_nat h1 gamma) /\
+    fmont_as_nat h1 alpha =
+      S.fmul (S.fmul 3 (S.fsub x (fmont_as_nat h1 delta))) (S.fadd x (fmont_as_nat h1 delta))))
 
-val lemma_point_abd: xD: int -> dlt: int ->
-  Lemma (3 * (xD - dlt) * (xD + dlt) == 3 * ((xD - dlt) * (xD + dlt)))
+let point_double_a_b_g_d p alpha beta gamma delta tmp =
+  let px = getx p in
+  let py = gety p in
+  let pz = getz p in
 
-let lemma_point_abd xD dlt = ()
+  let h0 = ST.get () in
+  fsqr pz delta;      // delta = z * z
+  fsqr py gamma;      // gamma = y * y
+  fmul px gamma beta; // beta = x * gamma
+  let h1 = ST.get () in
+  assert (fmont_as_nat h1 delta = S.fmul (fmont_as_nat h0 pz) (fmont_as_nat h0 pz));
+  assert (fmont_as_nat h1 gamma = S.fmul (fmont_as_nat h0 py) (fmont_as_nat h0 py));
+  assert (fmont_as_nat h1 beta = S.fmul (fmont_as_nat h0 px) (fmont_as_nat h1 gamma));
+
+  fsub px delta alpha;   // a0 = x - delta
+  let h2 = ST.get () in
+  assert (fmont_as_nat h2 alpha = S.fsub (fmont_as_nat h0 px) (fmont_as_nat h1 delta));
+  fmul_by_3 alpha tmp;
+  let h3 = ST.get () in
+  assert (fmont_as_nat h3 tmp = S.fmul 3 (fmont_as_nat h2 alpha));
+  fadd px delta alpha;   // a1 = x + delta
+  let h4 = ST.get () in
+  assert (fmont_as_nat h4 alpha = S.fadd (fmont_as_nat h0 px) (fmont_as_nat h1 delta));
+  fmul tmp alpha alpha
 
 
-let point_double_a_b_g p alpha beta gamma delta tempBuffer =
-  let pX = sub p (size 0) (size 4) in
-  let pY = sub p (size 4) (size 4) in
-  let pZ = sub p (size 8) (size 4) in
-
-  let a0 = sub tempBuffer (size 0) (size 4) in
-  let a1 = sub tempBuffer (size 4) (size 4) in
-  let alpha0 = sub tempBuffer (size 8) (size 4) in
-
-  fsqr pZ delta; (* delta = z * z*)
-  fsqr pY gamma; (* gamma = y * y *)
-  fmul pX gamma beta; (* beta = x * gamma *)
-
-  let h0 = ST.get() in
-
-  fsub pX delta a0; (* a0 = x - delta *)
-  fadd pX delta a1; (* a1 = x + delta *)
-  fmul a0 a1 alpha0; (* alpha = (x - delta) * (x + delta) *)
-  fmul_by_3 alpha0 alpha;
-
-    let xD = SM.from_mont (as_nat h0 pX) in
-    let dlt = SM.from_mont (as_nat h0 delta) in
-
-    calc (==)
-    {
-      (3 * (((xD - dlt) % S.prime) *  ((xD + dlt) % S.prime) % S.prime) % S.prime);
-    (==) {lemma_mod_mul_distr_l (xD - dlt) ((xD + dlt) % S.prime) S.prime; lemma_mod_mul_distr_r (xD - dlt) (xD + dlt) S.prime}
-      (3 * ((xD - dlt) *  (xD + dlt) % S.prime) % S.prime);
-    (==) {lemma_mod_mul_distr_r 3 ((xD - dlt) * (xD + dlt)) S.prime}
-      (3 * ((xD - dlt) * (xD + dlt)) % S.prime);
-    (==) {lemma_point_abd xD dlt}
-      (3 * (xD - dlt) * (xD + dlt)) % S.prime;
-  }
-
-val point_double_x3: x3: felem -> alpha: felem -> fourBeta: felem -> beta: felem -> eightBeta: felem ->
+inline_for_extraction noextract
+val point_double_x3: x3:felem -> alpha:felem -> beta:felem -> tmp:felem ->
   Stack unit
-    (requires fun h -> live h x3 /\ live h alpha /\ live h fourBeta /\ live h beta /\ live h eightBeta /\
-      LowStar.Monotonic.Buffer.all_disjoint [loc x3; loc alpha; loc fourBeta; loc beta; loc eightBeta] /\
-      as_nat h alpha < S.prime /\
-      as_nat h beta < S.prime
-    )
-    (ensures fun h0 _ h1 -> modifies (loc x3 |+| loc fourBeta |+| loc eightBeta) h0 h1 /\
-      as_nat h1 fourBeta = SM.to_mont (4 * SM.from_mont (as_nat h0 beta) % S.prime) /\
-      as_nat h1 x3 = SM.to_mont ((SM.from_mont (as_nat h0 alpha) * SM.from_mont (as_nat h0 alpha) - 8 * (SM.from_mont (as_nat h0 beta))) % S.prime)
-    )
+  (requires fun h ->
+    live h x3 /\ live h alpha /\ live h beta /\ live h tmp /\
+    LowStar.Monotonic.Buffer.all_disjoint
+      [loc x3; loc alpha; loc beta; loc tmp] /\
+    as_nat h alpha < S.prime /\ as_nat h beta < S.prime)
+  (ensures fun h0 _ h1 -> modifies (loc x3 |+| loc beta |+| loc tmp) h0 h1 /\
+    as_nat h1 beta < S.prime /\ as_nat h1 x3 < S.prime /\
+    fmont_as_nat h1 beta == S.fmul 4 (fmont_as_nat h0 beta) /\
+    fmont_as_nat h1 x3 == S.fsub (S.fmul (fmont_as_nat h0 alpha) (fmont_as_nat h0 alpha))
+      (S.fmul 8 (fmont_as_nat h0 beta)))
 
-let point_double_x3 x3 alpha fourBeta beta eightBeta  =
-    let h0 = ST.get() in
-  fsqr alpha x3; (* x3 = alpha ** 2 *)
-  fmul_by_4 beta fourBeta; (*  fourBeta = beta * 4 *)
-  fdouble fourBeta eightBeta; (* eightBeta = beta * 8 *)
-  fsub x3 eightBeta x3 (* x3 = alpha ** 2 - beta * 8 *);
-
-  calc(==)
-  {
-     SM.to_mont (((SM.from_mont (as_nat h0 alpha) * SM.from_mont (as_nat h0 alpha) % S.prime) - (2 *  (4 * SM.from_mont (as_nat h0 beta) % S.prime) % S.prime)) % S.prime);
-  (==) {lemma_mod_mul_distr_r 2 (4 * SM.from_mont (as_nat h0 beta)) S.prime}
-  SM.to_mont (((SM.from_mont (as_nat h0 alpha) * SM.from_mont (as_nat h0 alpha) % S.prime) - (8 * SM.from_mont (as_nat h0 beta)) % S.prime) % S.prime);
-  (==) {lemma_mod_sub_distr (SM.from_mont (as_nat h0 alpha) * SM.from_mont (as_nat h0 alpha) % S.prime) (8 * SM.from_mont (as_nat h0 beta)) S.prime}
-    SM.to_mont (((SM.from_mont (as_nat h0 alpha) * SM.from_mont (as_nat h0 alpha) % S.prime) - (8 * SM.from_mont (as_nat h0 beta))) % S.prime);
-  (==) {lemma_mod_add_distr (- 8 * SM.from_mont (as_nat h0 beta)) (SM.from_mont (as_nat h0 alpha) * SM.from_mont (as_nat h0 alpha)) S.prime}
-    SM.to_mont ((SM.from_mont (as_nat h0 alpha) * SM.from_mont (as_nat h0 alpha) - 8 * SM.from_mont (as_nat h0 beta)) % S.prime);
-  }
+let point_double_x3 x3 alpha beta tmp =
+  let h0 = ST.get () in
+  fsqr alpha x3;          // x3 = alpha * alpha
+  fmul_by_4 beta beta;    // beta = 4 * beta
+  let h1 = ST.get () in
+  assert (fmont_as_nat h1 x3 = S.fmul (fmont_as_nat h0 alpha) (fmont_as_nat h0 alpha));
+  assert (fmont_as_nat h1 beta = S.fmul 4 (fmont_as_nat h0 beta));
+  fdouble beta tmp;      // tmp = 8 * beta
+  let h2 = ST.get () in
+  assert (fmont_as_nat h2 tmp = S.fmul 2 (S.fmul 4 (fmont_as_nat h0 beta)));
+  Math.Lemmas.lemma_mod_mul_distr_r 2 (4 * fmont_as_nat h0 beta) S.prime;
+  assert (fmont_as_nat h2 tmp = S.fmul 8 (fmont_as_nat h0 beta));
+  fsub x3 tmp x3         // x3 = alpha * alpha - 8 * beta
 
 
-val point_double_z3: z3: felem -> pY: felem -> pZ: felem -> gamma: felem -> delta: felem ->
+inline_for_extraction noextract
+val point_double_z3: z3:felem -> py:felem -> pz:felem -> gamma:felem -> delta:felem ->
   Stack unit
-    (requires fun h -> live h z3 /\ live h pY /\ live h pZ /\ live h gamma /\ live h delta /\
-      eq_or_disjoint pZ z3 /\ disjoint z3 gamma /\ disjoint z3 delta /\ disjoint pY z3 /\
-      as_nat h gamma < S.prime /\
-      as_nat h delta < S.prime /\
-      as_nat h pY < S.prime /\
-      as_nat h pZ < S.prime
-    )
-    (ensures fun h0 _ h1 -> modifies (loc z3) h0 h1 /\
-      (
-	let y = SM.from_mont (as_nat h0 pY) in
-	let z = SM.from_mont (as_nat h0 pZ) in
-	as_nat h1 z3 = SM.to_mont (((y + z) * (y + z) - SM.from_mont (as_nat h0 gamma) - SM.from_mont (as_nat h0 delta)) % S.prime)
-      )
-    )
+  (requires fun h ->
+    live h z3 /\ live h py /\ live h pz /\ live h gamma /\ live h delta /\
+    eq_or_disjoint pz z3 /\ disjoint z3 gamma /\ disjoint z3 delta /\
+    disjoint py z3 /\ disjoint py pz /\
+    as_nat h gamma < S.prime /\ as_nat h delta < S.prime /\
+    as_nat h py < S.prime /\ as_nat h pz < S.prime)
+  (ensures fun h0 _ h1 -> modifies (loc z3) h0 h1 /\
+    as_nat h1 z3 < S.prime /\
+   (let yz = S.fadd (fmont_as_nat h0 py) (fmont_as_nat h0 pz) in
+    fmont_as_nat h1 z3 =
+      S.fsub (S.fsub (S.fmul yz yz) (fmont_as_nat h0 delta)) (fmont_as_nat h0 gamma)))
 
-let point_double_z3 z3 pY pZ gamma delta  =
-    let h0 = ST.get() in
+let point_double_z3 z3 py pz gamma delta =
+  let h0 = ST.get () in
+  fadd py pz z3;  // z3 = py + pz
+  fsqr z3 z3;     // z3 = (py + pz) * (py + pz)
+  let h1 = ST.get () in
+  assert (let yz = S.fadd (fmont_as_nat h0 py) (fmont_as_nat h0 pz) in
+    fmont_as_nat h1 z3 = S.fmul yz yz);
 
-  fadd pY pZ z3; (* z3 = py + pz *)
-  fsqr z3 z3; (* z3 = (py + pz) ** 2 *)
-  fsub z3 gamma z3; (* z3 =  (py + pz) ** 2 - gamma  *)
-  fsub z3 delta z3 (* z3 = (py + pz) ** 2 - gamma - delta *);
-
-    let pyD = SM.from_mont (as_nat h0 pY) in
-    let pzD = SM.from_mont (as_nat h0 pZ) in
-
-  calc (==)
-  {
-    SM.to_mont (((((( ((pyD + pzD) % S.prime) * ((pyD + pzD) % S.prime) % S.prime)) - SM.from_mont (as_nat h0 gamma)) % S.prime) - SM.from_mont (as_nat h0 delta)) % S.prime);
-  (==) {lemma_mod_mul_distr_l (pyD + pzD) ((pyD + pzD) % S.prime) S.prime; lemma_mod_mul_distr_r (pyD + pzD) (pyD + pzD) S.prime}
-    SM.to_mont ((((((pyD + pzD) * (pyD + pzD) % S.prime) - SM.from_mont (as_nat h0 gamma)) % S.prime) - SM.from_mont (as_nat h0 delta)) % S.prime);
-  (==) {lemma_mod_add_distr (- SM.from_mont (as_nat h0 gamma)) ((pyD + pzD) * (pyD + pzD)) S.prime }
-    SM.to_mont (((((pyD + pzD) * (pyD + pzD) - SM.from_mont (as_nat h0 gamma)) % S.prime) - SM.from_mont (as_nat h0 delta)) % S.prime);
-  (==) {lemma_mod_add_distr (- SM.from_mont (as_nat h0 delta)) ((pyD + pzD) * (pyD + pzD) - SM.from_mont (as_nat h0 gamma)) S.prime}
-    SM.to_mont (((pyD + pzD) * (pyD + pzD) - SM.from_mont (as_nat h0 gamma) - SM.from_mont (as_nat h0 delta)) % S.prime);
-  }
+  fsub z3 delta z3;  // z3 = (py + pz) ** 2 - delta
+  fsub z3 gamma z3   // z3 = (py + pz) ** 2 - delta - gamma
 
 
-val point_double_y3: y3: felem -> x3: felem -> alpha: felem -> gamma: felem -> eightGamma: felem -> fourBeta: felem ->
+inline_for_extraction noextract
+val point_double_y3: y3:felem -> x3:felem -> alpha:felem -> gamma:felem -> beta:felem ->
   Stack unit
-  (requires fun h -> live h y3 /\ live h x3 /\ live h alpha /\ live h gamma /\ live h eightGamma /\ live h fourBeta /\
-    LowStar.Monotonic.Buffer.all_disjoint [loc y3; loc x3; loc alpha; loc gamma; loc eightGamma; loc fourBeta] /\
-    as_nat h x3 < S.prime /\
-    as_nat h alpha < S.prime /\
-    as_nat h gamma < S.prime /\
-    as_nat h fourBeta < S.prime
-  )
-  (ensures fun h0 _ h1 -> modifies (loc y3 |+| loc gamma |+| loc eightGamma) h0 h1 /\
-    (
-      let alphaD = SM.from_mont (as_nat h0 alpha) in
-      let gammaD = SM.from_mont (as_nat h0 gamma) in
-      as_nat h1 y3 == SM.to_mont ((alphaD *  (SM.from_mont (as_nat h0 fourBeta) - SM.from_mont (as_nat h0 x3)) - 8 * gammaD * gammaD) % S.prime)
-    )
-  )
+  (requires fun h ->
+    live h y3 /\ live h x3 /\ live h alpha /\ live h gamma /\ live h beta /\
+    LowStar.Monotonic.Buffer.all_disjoint
+      [loc y3; loc x3; loc alpha; loc gamma; loc beta] /\
+    as_nat h x3 < S.prime /\ as_nat h alpha < S.prime /\
+    as_nat h gamma < S.prime /\ as_nat h beta < S.prime)
+  (ensures fun h0 _ h1 -> modifies (loc y3 |+| loc gamma) h0 h1 /\
+    as_nat h1 y3 < S.prime /\
+    fmont_as_nat h1 y3 ==
+    S.fsub
+      (S.fmul (fmont_as_nat h0 alpha) (S.fsub (fmont_as_nat h0 beta) (fmont_as_nat h0 x3)))
+      (S.fmul (S.fmul 8 (fmont_as_nat h0 gamma)) (fmont_as_nat h0 gamma)))
+
+let point_double_y3 y3 x3 alpha gamma beta =
+  let h0 = ST.get () in
+  fsub beta x3 y3;      // y3 = beta - x3
+  fmul alpha y3 y3;     // y3 = alpha * (beta - x3)
+  let h1 = ST.get () in
+  assert (fmont_as_nat h1 y3 =
+    S.fmul (fmont_as_nat h0 alpha) (S.fsub (fmont_as_nat h0 beta) (fmont_as_nat h0 x3)));
+
+  fsqr gamma gamma;
+  fmul_by_8 gamma gamma; // gamma = 8 * gamma * gamma
+  let h2 = ST.get () in
+  assert (let g = fmont_as_nat h0 gamma in
+    fmont_as_nat h2 gamma == S.fmul 8 (S.fmul g g));
+  Lib.NatMod.lemma_mul_mod_assoc #S.prime 8 (fmont_as_nat h0 gamma) (fmont_as_nat h0 gamma);
+  fsub y3 gamma y3       // y3 = alpha * (beta - x3) - 8 * gamma * gamma
 
 
+[@CInline]
+let point_double p res tmp =
+  let px = getx p in
+  let py = gety p in
+  let pz = getz p in
 
-let point_double_y3 y3 x3 alpha gamma eightGamma fourBeta =
-    let h0 = ST.get() in
-  fsub fourBeta x3 y3; (* y3 = 4 * beta - x3 *)
-  fmul alpha y3 y3; (* y3 = alpha * (4 * beta - x3) *)
-  fsqr gamma gamma; (* gamma = gamma ** 2 *)
-  fmul_by_8 gamma eightGamma; (* gamma = 8 * gamma ** 2 *)
-  fsub y3 eightGamma y3; (* y3 = alpha * y3 - 8 * gamma **2 *)
+  let x3 = getx res in
+  let y3 = gety res in
+  let z3 = getz res in
 
+  let delta = sub tmp 0ul 4ul in
+  let gamma = sub tmp 4ul 4ul in
+  let beta  = sub tmp 8ul 4ul in
+  let alpha = sub tmp 12ul 4ul in
+  let ftmp  = sub tmp 16ul 4ul in
 
-  let alphaD = SM.from_mont (as_nat h0 alpha) in
-  let gammaD = SM.from_mont (as_nat h0 gamma) in
-
-  calc(==)
-  {
-     SM.to_mont (((SM.from_mont (as_nat h0 alpha) *  ((SM.from_mont (as_nat h0 fourBeta) - SM.from_mont (as_nat h0 x3)) % S.prime) % S.prime) - (8 *  (SM.from_mont (as_nat h0 gamma) * SM.from_mont (as_nat h0 gamma) % S.prime) % S.prime)) % S.prime);
-  (==) {lemma_mod_mul_distr_r (SM.from_mont (as_nat h0 alpha)) (((SM.from_mont (as_nat h0 fourBeta) - SM.from_mont (as_nat h0 x3)))) S.prime}
-    SM.to_mont (((SM.from_mont (as_nat h0 alpha) *  (SM.from_mont (as_nat h0 fourBeta) - SM.from_mont (as_nat h0 x3)) % S.prime) - (8 *  (SM.from_mont (as_nat h0 gamma) * SM.from_mont (as_nat h0 gamma) % S.prime) % S.prime)) % S.prime);
-  (==) {lemma_mod_mul_distr_r 8 (SM.from_mont (as_nat h0 gamma) * (SM.from_mont (as_nat h0 gamma))) S.prime}
-    SM.to_mont (((alphaD *  (SM.from_mont (as_nat h0 fourBeta) - SM.from_mont (as_nat h0 x3)) % S.prime) - (8 * (gammaD * gammaD) % S.prime)) % S.prime);
-  (==) {lemma_mod_add_distr (-(8 * (gammaD * gammaD) % S.prime)) (alphaD *  (SM.from_mont (as_nat h0 fourBeta) - SM.from_mont (as_nat h0 x3))) S.prime  }
-      SM.to_mont (((alphaD *  (SM.from_mont (as_nat h0 fourBeta) - SM.from_mont (as_nat h0 x3))) - (8 * (gammaD * gammaD) % S.prime)) % S.prime);
-  (==) {lemma_mod_sub_distr (alphaD *  (SM.from_mont (as_nat h0 fourBeta) - SM.from_mont (as_nat h0 x3))) (8 * (gammaD * gammaD)) S.prime}
-       SM.to_mont (((alphaD *  (SM.from_mont (as_nat h0 fourBeta) - SM.from_mont (as_nat h0 x3))) - (8 * (gammaD * gammaD))) % S.prime);
-  (==) {assert_by_tactic (8 * (gammaD * gammaD) == 8 * gammaD * gammaD) canon}
-    SM.to_mont ((alphaD *  (SM.from_mont (as_nat h0 fourBeta) - SM.from_mont (as_nat h0 x3)) - 8 * gammaD * gammaD) % S.prime);
-}
-
-
-val lemma_pd_to_spec: x: nat -> y: nat -> z: nat -> x3: nat -> y3: nat -> z3: nat ->  Lemma
-  (requires (
-    let xD, yD, zD = SM.from_mont x, SM.from_mont y, SM.from_mont z in
-    x3 == SM.to_mont (((3 * (xD - zD * zD) * (xD + zD * zD)) * (3 * (xD - zD * zD) * (xD + zD * zD)) - 8 * xD * (yD * yD)) % S.prime) /\
-    y3 == SM.to_mont ((3 * (xD - zD * zD) * (xD + zD * zD) *  (4 * xD * (yD * yD) - SM.from_mont x3) - 8 * (yD * yD) * (yD * yD)) % S.prime) /\
-    z3 = SM.to_mont (((yD + zD) * (yD + zD) - zD * zD - yD * yD) % S.prime)
-  )
-)
- (ensures(
-   let xD, yD, zD = SM.from_mont x, SM.from_mont y, SM.from_mont z in
-   let x3D, y3D, z3D = SM.from_mont x3, SM.from_mont y3, SM.from_mont z3 in
-   let xN, yN, zN = S.point_double (xD, yD, zD) in
-   x3D == xN /\ y3D == yN /\ z3D == zN))
-
-let lemma_pd_to_spec x y z x3 y3 z3 =
-  let xD, yD, zD = SM.from_mont x, SM.from_mont y, SM.from_mont z in
-  let x3D, y3D, z3D = SM.from_mont x3, SM.from_mont y3, SM.from_mont z3 in
-  assert(let xN, yN, zN = S.point_double (xD, yD, zD) in
-      x3D == xN /\ y3D == yN /\ z3D == zN)
-
-
-
-let point_double p result tempBuffer =
-  let pX = sub p (size 0) (size 4) in
-  let pY = sub p (size 4) (size 4) in
-  let pZ = sub p (size 8) (size 4) in
-
-  let x3 = sub result (size 0) (size 4) in
-  let y3 = sub result (size 4) (size 4) in
-  let z3 = sub result (size 8) (size 4) in
-
-  let delta = sub tempBuffer (size 0) (size 4) in
-  let gamma = sub tempBuffer (size 4) (size 4) in
-  let beta = sub tempBuffer (size 8) (size 4) in
-  let alpha = sub tempBuffer (size 16) (size 4) in
-
-  let fourBeta = sub tempBuffer (size 20) (size 4) in
-  let eightBeta = sub tempBuffer (size 24) (size 4) in
-  let eightGamma = sub tempBuffer (size 28) (size 4) in
-
-  let tmp = sub tempBuffer (size 32) (size 12) in
-
-
-  let h0 = ST.get() in
-    point_double_a_b_g p alpha beta gamma delta tmp;
-    point_double_x3 x3 alpha fourBeta beta eightBeta;
-    point_double_z3 z3 pY pZ gamma delta;
-    point_double_y3 y3 x3 alpha gamma eightGamma fourBeta;
-
-  let h4 = ST.get() in
-
-  let x = SM.from_mont (as_nat h0 (gsub p (size 0) (size 4))) in
-  let y = SM.from_mont (as_nat h0 (gsub p (size 4) (size 4))) in
-  let z = SM.from_mont (as_nat h0 (gsub p (size 8) (size 4))) in
-
-  lemma_x3 x y z;
-  lemma_z3 x y z;
-  lemma_y3 x y z (SM.from_mont (as_nat h4 x3));
-  lemma_pd_to_spec
-    (as_nat h0 (gsub p (size 0) (size 4)))
-      (as_nat h0 (gsub p (size 4) (size 4)))
-	(as_nat h0 (gsub p (size 8) (size 4)))
-    (as_nat h4 (gsub result (size 0) (size 4)))
-      (as_nat h4 (gsub result (size 4) (size 4)))
-	(as_nat h4 (gsub result (size 8) (size 4)))
+  point_double_a_b_g_d p alpha beta gamma delta ftmp;
+  point_double_x3 x3 alpha beta ftmp;
+  point_double_z3 z3 py pz gamma delta;
+  point_double_y3 y3 x3 alpha gamma beta
